DeBruijnSSA/BinSyntax/Rewrite/Term/Induction.lean
@@ -1,4 +1,4 @@
-import DeBruijnSSA.BinSyntax.Rewrite.Term.Setoid
+import DeBruijnSSA.BinSyntax.Rewrite.Term.Eqv
 
 import Discretion.Utils.Quotient
 
@@ -8,5 +8,36 @@ variable [Φ: EffInstSet φ (Ty α) ε] [PartialOrder α] [SemilatticeSup ε] [O
 
 namespace Term
 
-
--- ...
+theorem Eqv.induction
+  {motive : (Γ : Ctx α ε) → (V : Ty α × ε) → Eqv φ Γ V → Prop}
+  (var : ∀{Γ V} (n) (hv : Γ.Var n V), motive Γ V (var n hv))
+  (op : ∀{Γ A B e} (f a) (hf : Φ.EFn f A B e) (_ha : motive Γ ⟨A, e⟩ a),
+    motive Γ ⟨B, e⟩ (op f hf a))
+  (let1 : ∀{Γ A B e} (a b) (_ha : motive Γ ⟨A, e⟩ a) (_hb : motive (⟨A, ⊥⟩::Γ) ⟨B, e⟩ b),
+    motive Γ ⟨B, e⟩ (let1 a b))
+  (pair : ∀{Γ A B e} (a b) (_ha : motive Γ ⟨A, e⟩ a) (_hb : motive Γ ⟨B, e⟩ b),
+    motive Γ ⟨Ty.prod A B, e⟩ (pair a b))
+  (let2 : ∀{Γ A B C e} (a c)
+    (_ha : motive Γ ⟨A.prod B, e⟩ a) (_hc : motive (⟨B, ⊥⟩::⟨A, ⊥⟩::Γ) ⟨C, e⟩ c),
+    motive Γ ⟨C, e⟩ (let2 a c))
+  (inl : ∀{Γ A B e} (a) (_ha : motive Γ ⟨A, e⟩ a), motive Γ ⟨Ty.coprod A B, e⟩ (inl a))
+  (inr : ∀{Γ A B e} (b) (_hb : motive Γ ⟨B, e⟩ b), motive Γ ⟨Ty.coprod A B, e⟩ (inr b))
+  (case : ∀{Γ A B C e} (a l r)
+    (_ha : motive Γ ⟨Ty.coprod A B, e⟩ a)
+    (_hl : motive (⟨A, ⊥⟩::Γ) ⟨C, e⟩ l)
+    (_hr : motive (⟨B, ⊥⟩::Γ) ⟨C, e⟩ r),
+    motive Γ ⟨C, e⟩ (case a l r))
+  (abort : ∀{Γ A e} (a) (_ha : motive Γ ⟨Ty.empty, e⟩ a), motive Γ ⟨A, e⟩ (abort a A))
+  (unit : ∀{Γ e}, motive Γ ⟨Ty.unit, e⟩ (unit e))
+  (h : Eqv φ Γ V) : motive Γ V h := by induction h using Quotient.inductionOn with
+  | h a => induction a using InS.induction with
+  | var n hv => exact var n hv
+  | op f a hf Ia => exact op f ⟦a⟧ hf Ia
+  | let1 a b Ia Ib => exact let1 ⟦a⟧ ⟦b⟧ Ia Ib
+  | pair a b Ia Ib => exact pair ⟦a⟧ ⟦b⟧ Ia Ib
+  | let2 a c Ia Ic => exact let2 ⟦a⟧ ⟦c⟧ Ia Ic
+  | inl a Ia => exact inl ⟦a⟧ Ia
+  | inr b Ib => exact inr ⟦b⟧ Ib
+  | case a l r Ia Il Ir => exact case ⟦a⟧ ⟦l⟧ ⟦r⟧ Ia Il Ir
+  | abort a Ia => exact abort ⟦a⟧ Ia
+  | unit => exact unit
